WIP state modeling

src/State.v
@@ -1,13 +1,68 @@
 Require Import QHTT.Axioms.
 Require Import Arith.
 
+(* location or label to refer to a qubit *)
 Definition loc := nat.
 Definition val := dynamic%type.
 
+(* state is a partial function from locations to dynamic
+  (that stores both type and value, ie, abstracted type) *)
 Definition state := loc -> option val.
 
+(** * Useful state assertions *)
 
 Definition empty : state := fun _ => None.
 
 Definition singleton (l : loc) (v : val) : state :=
   fun l' => if eq_nat_dec l l' then Some v else None.
+
+(* qubit initialization (assuming value is a qubit)
+   TODO support converting from a bool here? *)
+Definition init (s : state) (l : loc) (v : val) : state :=
+  fun l' => if eq_nat_dec l l' then Some v else s l'.
+
+(* measurement, currently returns whatever representation is stored *)
+Definition meas (s : state) (l : loc) : option val :=
+  s l.
+
+(* no equivalent of free needed here? *)
+
+Infix "|-->" := singleton (at level 35, no associativity).
+
+Definition join (s1 s2 : state) : state :=
+  fun l => match s1 l with
+        | None => s2 l
+        | v => v
+        end.
+
+Infix "*" := join (at level 40, left associativity).
+
+(** * Some theorems *)
+
+Theorem join_id1 : forall s, empty * s = s.
+  intros s.
+  unfold join. simpl.
+  ext_eq. reflexivity.
+Qed.
+
+
+Theorem join_id2 : forall s, s * empty = s.
+  intros s.
+  unfold join.
+  ext_eq.
+  destruct (s x).
+  - reflexivity.
+  - unfold empty. reflexivity.
+Qed.
+
+Hint Resolve join_id2 join_id1 : QHTT.
+Hint Rewrite join_id2 join_id1 : QHTT.
+
+Theorem meas_empty : forall l,
+    (meas empty l) = None.
+  intros l.
+  unfold meas. unfold empty.
+  reflexivity.
+Qed.
+
+
